chore: add register allocation only for constants

SSA/Projects/Regalloc/RegallocSingleBB.lean
@@ -1,26 +1,24 @@
 -- Register allocation for a single basic block program.
 import SSA.Core.Framework
+import Lean.Data.HashMap
 
 namespace Pure
 
-inductive BinopKind
-| add 
-
-inductive Op 
-| binop (binopKind : BinopKind)
+inductive Op
+| add
 | const (i : Int)
 
-inductive Ty 
+inductive Ty
 -- | int (width : Nat) : Ty
 | int : Ty
 
 
-abbrev dialect : Dialect where 
+abbrev dialect : Dialect where
  Op := Op
  Ty := Ty
 
 def Op.signature : Op → Signature Ty
-| .binop .add => {
+| .add => {
     sig := [.int, .int],
     regSig := .nil,
     outTy := .int
@@ -31,14 +29,153 @@ def Op.signature : Op → Signature Ty
     outTy := .int
   }
 
+
+instance : TyDenote Ty where
+   toType := fun
+    | .int => Int
+
  instance : DialectSignature dialect where
    signature := Op.signature
+
+instance : DialectDenote dialect where
+  denote := fun op args _ =>
+  match op with
+  | .add =>
+    let l : Int := args.getN 0
+    let r : Int := args.getN 1
+    l + r
+  | .const i => i
+
+ def Program (Γ Δ : Ctxt Ty) : Type := Lets dialect Γ .pure Δ
+
  end Pure
 
 
-
  namespace RegAlloc
+
+ def Reg := Nat
+ deriving DecidableEq, Repr, Inhabited, BEq
+
+ abbrev RegisterFile : Type := Reg → Int
+def RegisterFile.get (R : RegisterFile) (r : Reg) : Int := R r
+ def RegisterFile.set (R : RegisterFile) (r : Reg) (v : Int) : RegisterFile :=
+  fun r' => if r = r' then v else R r'
+
+inductive Op
+| add (l r out : Reg)
+| const (i : Int) (out : Reg)
+
+inductive Ty
+| unit : Ty
+
+abbrev dialect : Dialect where
+  Op := Op
+  Ty := Ty
+  m := StateM RegisterFile
+
+def Op.signature : Op → Signature Ty
+| .add _ _ _ => {
+    sig := [],
+    regSig := .nil,
+    outTy := .unit,
+    effectKind := .impure
+  }
+| .const _x _  => {
+    sig := []
+    regSig := .nil,
+    outTy := .unit,
+    effectKind := .impure
+  }
+
+ instance : DialectSignature dialect where
+   signature := Op.signature
+
+instance : TyDenote Ty where
+   toType := fun
+    | .unit => Unit
+
+ instance : DialectSignature dialect where
+   signature := Op.signature
+
+def readRegister (r : Reg) : StateM RegisterFile Int := fun R => (R r, R)
+def writeRegister (r : Reg) (v : Int) : StateM RegisterFile Unit := fun R => ((), R.set r v)
+
+instance : DialectDenote dialect where
+  denote := fun op _ _ =>
+  match op with
+  | .add l r rout => show StateM _ _ from
+     readRegister l >>= fun vl =>
+     readRegister r >>= fun vr =>
+     writeRegister rout (vl + vr)
+  | .const i rout => show StateM _ _ from
+     writeRegister rout i
+
+ def Program (Γ Δ : Ctxt Ty) : Type := Lets dialect Γ .impure Δ
+
  end RegAlloc
-  
-#check Dialect
-#check Lets
+
+
+/-- A mapping of variables in a context to a register. -/
+structure RegisterMap (Γ : Ctxt Pure.Ty) where
+  toFun : Γ.Var Pure.Ty.int → RegAlloc.Reg -- I actually want a partial function here.
+  live : List RegAlloc.Reg -- TODO: move to using HashMap once available for HashSet.
+  -- hlive : ∀ r ∈ live, ∃ v, toFun v = r -- every live register is mapped to a variable.
+  -- hinjective : Injective toFun
+
+ /--
+ A correspondence between variables 'v ∈ Γ' and registers in the register file.
+ This correspondence is witnessed by 'f'.
+ -/
+ def correspondence {Γ : Ctxt Pure.Ty} (V : Γ.Valuation) (f : RegisterMap Γ) (R : RegAlloc.RegisterFile) : Prop :=
+  ∀ (v : Γ.Var Pure.Ty.int), R (f.toFun v) = V v
+
+/-- All register files correspond to the start of the program. -/
+theorem correspondence_nil (R : RegAlloc.RegisterFile) :
+    correspondence (Γ := []) V f R := by
+  intros v
+  exact v.emptyElim
+
+
+/--
+For a sequence of lets [v1 := e1, ..., vn := en, vn+1 := en+1], clear the register assigned to 'vn+1' and return it.
+-/
+def RegisterMap.lookupAndDeleteLast {Γ : Ctxt Pure.Ty} {t : Pure.Ty} (f : RegisterMap <| Γ.snoc t) : RegAlloc.Reg × RegisterMap Γ :=
+  let vlast := Ctxt.Var.last Γ t
+  let r := f.toFun vlast
+  (r, {
+    toFun := fun v => f.toFun (v.toSnoc),
+    live := f.live.erase (f.toFun <| Ctxt.Var.last Γ t) -- state that this register is now killed.
+  })
+
+
+/--
+Convert a pure context to an impure context, where all SSA variables are now side effecting, and thus
+have type ().
+-/
+def doRegAllocCtx (ctx : Ctxt Pure.Ty) : Ctxt RegAlloc.Ty := ctx.map (fun _ => RegAlloc.Ty.unit)
+
+@[simp]
+theorem doRegAllocCtx_nil : doRegAllocCtx [] = [] := rfl
+
+@[simp]
+def doRegAllocCtx_cons : doRegAllocCtx (Γ.snoc s) = (doRegAllocCtx Γ).snoc RegAlloc.Ty.unit := rfl
+
+def doRegAllocExpr (f : RegisterMap (Γ.snoc s))
+  (e : Expr Pure.dialect Γ EffectKind.pure .int) :
+  Expr RegAlloc.dialect (doRegAllocCtx Γ) EffectKind.impure .unit × RegisterMap Γ :=
+  match e.op with
+  | .const i =>
+      let (r, f) := f.lookupAndDeleteLast
+      (Expr.mk (RegAlloc.Op.const i r) rfl (by simp) .nil .nil, f)
+  | .add => sorry
+
+/-- TODO: we will get stuck in showing that 'nregs > 0' when we decrement it when a variable is defined (ie, dies in reverse order).
+This might have us actually need to compute liveness anyway to prove correctness.
+-/
+def doRegAllocLets (f : RegisterMap Δ) (p : Pure.Program Γ Δ) : RegAlloc.Program (doRegAllocCtx Γ) (doRegAllocCtx Δ) × RegisterMap Γ :=
+  match p with
+  | .nil => (.nil, f)
+  | .var ps e (Γ_out := Ξ) (t := t) =>
+    let (er, f) := doRegAllocExpr f e
+    let (psr, f) := doRegAllocLets f ps
+    (.var psr er, f)
